Fancier Automation working for everything but TCP example.

src/Narcissus/Formats/Base/SequenceFormat.v
@@ -19,30 +19,24 @@ Section SequenceFormat.
     := (fun s => compose _ (format1 s) (format2 s))%comp.
 
   Definition sequence_Decode
-             {S S' : Type}
+             {S S' T : Type}
+             {cache : Cache}
              (decode1 : DecodeM (S' * T) T)
-             (decode2 : S' -> DecodeM S T)
-    : DecodeM S T
-    := (fun t env =>
-          match decode1 t env with
-          | Some (s', t', env') => decode2 s' t' env'
-          | None => None
-          end).
+             (decode2 : S' -> DecodeM (S * T) T)
+    : DecodeM (S * T) T :=
+    fun t env =>
+      `(s', t', env') <- decode1 t env;
+        decode2 s' t' env'.
 
   Definition sequence_Decode'
              {S S' : Type}
              (decode1 : DecodeM (S' * T) T)
              (decode2 : S' -> DecodeM (S * T) T)
     : DecodeM (S' * S * T) T :=
-    fun t env =>
-      match decode1 t env with
-      | Some (s', t', env') =>
-        match decode2 s' t' env' with
-        | Some (s, t', env'') => Some ((s', s), t', env'')
-        | None => None
-        end
-      | None => None
-      end.
+      fun t env =>
+      `(s', t', env') <- decode1 t env;
+      `(s, t', env'') <- decode2 s' t' env';
+      Some ((s', s), t', env'').
 
   Definition sequence_Encode
              {S : Type}
@@ -108,12 +102,6 @@ Section SequenceFormat.
         (format1 format2 : FormatM S T )
         (decode1 : DecodeM (V1 * T) T)
         (view_format1 : FormatM V1 T)
-        (consistency_predicate_OK :
-           forall s v1 t1 t2 env xenv xenv',
-             computes_to (format1 s env) (t1, xenv)
-             -> computes_to (view_format1 v1 env) (t2, xenv')
-             -> view1 s v1
-             -> consistency_predicate v1 s)
       (*consistency_predicate_refl :
          forall a, consistency_predicate (proj' a) (proj a))
       (proj_predicate_OK :
@@ -123,6 +111,13 @@ Section SequenceFormat.
          cache_inv_Property P P_inv1
          -> CorrectDecoder monoid Source_Predicate View_Predicate1 view1 format1 decode1 P view_format1)
       (*pred_pf : forall s, predicate s -> predicate' s *)
+      (consistency_predicate_OK :
+         forall s v1 t1 t2 env xenv xenv',
+           computes_to (format1 s env) (t1, xenv)
+           -> computes_to (view_format1 v1 env) (t2, xenv')
+           -> view1 s v1
+           -> consistency_predicate v1 s)
+
       (decode2 : V1 -> DecodeM (V2 * T) T)
       (view_format2 : V1 -> FormatM V2 T)
       (view_format3 : FormatM (V1 * V2) T)
@@ -153,7 +148,7 @@ Proof.
     unfold compose, Bind2 in com_pf; computes_to_inv; destruct v;
       destruct v0.
     destruct (fun H => proj1 (decode1_pf (proj1 P_inv_pf)) _ _ _ _ _ (mappend t1 ext) env_OK env_pm H com_pf); eauto; destruct_ex; split_and; simpl in *; injections; eauto.
-    unfold sequence_Decode'.
+    unfold sequence_Decode', DecodeBindOpt2, BindOpt.
     setoid_rewrite <- mappend_assoc; rewrite H0.
     pose proof (proj2 (decode1_pf H2) _ _ _ _ _ _ env_pm env_OK H0);
       split_and; destruct_ex; split_and.
@@ -162,10 +157,11 @@ Proof.
     split; try eassumption.
     eauto.
     destruct_ex; split_and.
-    rewrite H11; eexists _, _; eauto.
+    simpl.
+    rewrite H11; eexists _, _; simpl; eauto.
   }
   { intros ? ? ? ? t; intros.
-    unfold sequence_Decode' in H1.
+    unfold sequence_Decode', DecodeBindOpt2, BindOpt in H1.
     destruct (decode1 t env') as [ [ [? ?] ? ] | ] eqn : ? ;
       simpl in *; try discriminate.
     generalize Heqo; intros Heqo'.
@@ -185,69 +181,6 @@ Proof.
     apply unfold_computes; eassumption.
   }
 Qed.
-
-  (*Corollary CorrectDecoder_sequence_Done
-            {S : Type}
-            (P : S -> Prop)
-            (format : FormatM (S * T) T)
-            (s : S)
-            (singleton_format : forall (s' : S) (t : T) env tenv',
-                format (s', t) env ∋ tenv' <-> s' = s
-                                               /\ fst tenv' = mempty
-                                               /\ snd tenv' = env)
-    : CorrectDecoder_simpl (format ++ ?* ) (LaxTerminal_Decode s).
-  Proof.
-    unfold CorrectDecoder_simpl, LaxTerminal_Format,
-    LaxTerminal_Decode, sequence_Format, Compose_Format; split; intros.
-    - unfold Bind2 in H0; computes_to_inv; subst.
-      injections.
-      destruct data; eapply singleton_format in H0; simpl in *; intuition; subst.
-      destruct v; simpl in *; subst.
-      eexists; split; eauto.
-      rewrite mempty_left; reflexivity.
-    - injections; unfold Bind2; eexists.
-
-      simpl.
-      destruct v; destruct v0; simpl in *; injections.
-      destruct decode1_correct as [? _].
-      destruct (decode2_correct x) as [? _].
-      destruct (H0 env env' c (x, t0) (mappend t t0)) as (xenv', (decode1_eq, Equiv_xenv));
-        eauto.
-      rewrite decode1_eq; eauto.
-      eapply H3; eauto.
-      unfold Restrict_Format, Compose_Format; apply unfold_computes.
-      setoid_rewrite unfold_computes; eexists; intuition eauto.
-    - destruct (decode1 bin env') as [ [ [s' t'] xenv'']  | ] eqn: ?; try discriminate.
-      destruct decode1_correct as [decode1_correct' decode1_correct].
-      specialize (decode2_correct s'); destruct decode2_correct as [_ decode2_correct].
-      generalize Heqo; intro Heqo'.
-      eapply decode1_correct in Heqo; eauto.
-      destruct_ex; split_and.
-      eapply decode2_correct in H0; eauto.
-      destruct_ex; split_and.
-      eexists; intuition eauto.
-      unfold Restrict_Format, Compose_Format, LaxTerminal_Format, sequence_Format,
-        Bind2 in *; computes_to_inv.
-      rewrite @unfold_computes in H1.
-      destruct_ex; split_and; simpl in *; subst.
-      eapply format1'_overlap in H2; destruct_ex; split_and; subst; eauto.
-  Qed.
-    unfold
-
-    eapply (CorrectDecoder_sequence (fun s s' => f s = s')); eauto; intros;
-      unfold Projection_Format, Compose_Format, sequence_Format, Bind2, LaxTerminal_Format in *.
-    - rewrite @unfold_computes in H.
-      destruct_ex; split_and; subst.
-      eexists; intros; intuition.
-      destruct tenv'; simpl; computes_to_econstructor.
-      rewrite unfold_computes; eauto.
-      simpl; computes_to_econstructor; eauto.
-    - computes_to_inv; subst.
-      apply_in_hyp @unfold_computes; destruct_ex; split_and; subst.
-      eexists; simpl; intuition eauto.
-      destruct v; apply unfold_computes; eauto.
-  Qed. *)
-
 
 End SequenceFormat.
 
