src/Narcissus/Examples/NetworkStack/UDP_Packet.v
@@ -83,18 +83,6 @@ Section UDP_Decoder.
   (* Step Two and a Half: Add some simple facts about correct packets
    for the decoder automation. *)
 
-  Lemma CorrectDecoder_foo s len_format1 len_format2 :
-    CorrectDecoderFor (fun n => n = len_format1 s + len_format2 s + 16) (fun n : nat => UDP_Packet_Format s).
-    unfold UDP_Packet_Format.
-    eapply Start_CorrectDecoderFor.
-    apply_rules.
-
-    start_synthesizing_decoder.
-    econstructor.
-
-
-    (format1 ++ format_unused_word 16 ++ format2)%format decodeA P) ->
-
   Lemma UDP_Packet_Header_Len_OK
     : forall (a : UDP_Packet) (ctx ctx' ctx'' : CacheFormat) (c : word 16) (b b'' ext : ByteString),
       (format_word ◦ SourcePort ++ format_word ◦ DestPort ++ format_nat 16 ◦ Init.Nat.add 8 ∘ (projT1 (P:=ByteBuffer.t) ∘ Payload)) a
@@ -165,7 +153,7 @@ Section UDP_Decoder.
     match goal with
     | |- _ => intros; eapply unused_word_decode_correct; eauto
     | H : cache_inv_Property ?mnd _
-      |- CorrectDecoder _ _ _ (?fmt1 ThenChecksum _ OfSize _ ThenCarryOn ?format2) _ _ =>
+      |- CorrectDecoder _ _ _ _ (?fmt1 ThenChecksum _ OfSize _ ThenCarryOn ?format2) _ _ _ =>
       eapply compose_PseudoChecksum_format_correct;
       [ repeat calculate_length_ByteString
       | repeat calculate_length_ByteString
@@ -175,7 +163,7 @@ Section UDP_Decoder.
       | apply UDP_Packet_Header_Len_OK
       | intros; NormalizeFormats.normalize_format ]
     | H : cache_inv_Property ?mnd _
-      |- CorrectDecoder _ _ _ format_bytebuffer _ _ =>
+      |- CorrectDecoder _ _ _ _ format_bytebuffer _ _ _ =>
       intros; eapply @ByteBuffer_decode_correct;
       first [exact H | solve [intros; intuition eauto] ]
   end.
